Verify queue pop function, with Son
Also add some comments and tweaks to queueProgScript.sml

characteristic/examples/queueProgScript.sml
@@ -1,4 +1,11 @@
-open  preamble ml_progLib ioProgLib ml_translatorLib
+(*
+
+An example of a queue data structure implemented using CakeML arrays, verified
+using CF.
+
+*)
+
+open  preamble ml_progLib ml_translatorLib
       cfTacticsLib basisFunctionsLib ml_translatorTheory
 
 val _ = new_theory "queueProg";
@@ -7,33 +14,44 @@ val _ = translation_extends"ioProg";
 
 val queue_decls = process_topdecs
     `fun empty_queue u = ref (Array.arrayEmpty (), 0)
-    
+
     fun push q e =
     	case !q of (a,i) =>
-	let val l = Array.length a in
-      	if i >= l then
-      	   let val a' = Array.array (2*l+1) e in
-	   (Array.copy a a' 0;
-	   q := (a', i+1))
-	   end
+      let val l = Array.length a in
+        if i >= l then
+          let val a' = Array.array (2*l+1) e in
+            (Array.copy a a' 0;
+             q := (a', i+1))
+          end
       	else
-	   (Array.update a i e; q := (a,i+1))
-	end
+          (Array.update a i e;
+           q := (a,i+1))
+      end
 
     exception EmptyQueue
-  
+
     fun pop q =
     	case !q of (a,i) =>
       	if i = 0 then raise EmptyQueue
-      	else let val e = Array.sub a (i-1) in (q := (a, i-1); e) end`
-	
-val _ = append_prog queue_decls
+      	else let val x = Array.sub a (i-1) in (q := (a, i-1); x) end`;
 
+val _ = append_prog queue_decls;
+
+val EmptyQueue_exn_def = Define`
+  EmptyQueue_exn v = (v = Conv (SOME ("EmptyQueue", TypeExn (Short "EmptyQueue"))) [])`;
+
+(* Heap predicate for queues:
+   QUEUE A vs qv means qv is a reference to a queue of
+   elements vs which satisfy A *)
 val QUEUE_def  = Define `
   QUEUE A vs qv =
-  SEP_EXISTS av iv vvs junk. REF qv (Conv NONE [av;iv]) * & NUM (LENGTH vs) iv * ARRAY av (vvs ++ junk) * & LIST_REL A vs vvs`
+  SEP_EXISTS av iv vvs junk.
+    REF qv (Conv NONE [av;iv]) *
+    & NUM (LENGTH vs) iv *
+    ARRAY av (vvs ++ junk) *
+    & LIST_REL A vs vvs`;
 
-val st = get_ml_prog_state ()
+val st = get_ml_prog_state ();
 
 val empty_queue_spec = Q.store_thm ("empty_queue_spec",
     `!uv. app (p:'ffi ffi_proj) ^(fetch_v "empty_queue" st) [uv]
@@ -45,8 +63,7 @@ val empty_queue_spec = Q.store_thm ("empty_queue_spec",
       &(pv = Conv NONE [av; iv]) * ARRAY av [] * &NUM 0 iv`
     THEN1(xcon \\ xsimpl) \\
     xapp \\ xsimpl \\ simp[QUEUE_def] \\ xsimpl
-)
-
+);
 
 val push_spec = Q.store_thm ("push_spec",
     `!qv xv vs x. app (p:'ffi ffi_proj) ^(fetch_v "push" st) [qv; xv]
@@ -63,7 +80,7 @@ val push_spec = Q.store_thm ("push_spec",
     >> xif
     >- (
        imp_res_tac LIST_REL_LENGTH >> fs[]
-       >> `LENGTH junk = 0` by decide_tac >> 
+       >> `LENGTH junk = 0` by decide_tac >>
        xlet `POSTv nlv. & NUM (2* (LENGTH vs)) nlv * qv ~~> Conv NONE [av; iv] * ARRAY av (vvs ++ junk)`
        >- (xapp >> xsimpl >> fs[NUM_def] >> instantiate) >>
        xlet `POSTv nlv. & NUM (2* (LENGTH vs) + 1) nlv * qv ~~> Conv NONE [av; iv] * ARRAY av (vvs ++ junk)`
@@ -94,7 +111,6 @@ val push_spec = Q.store_thm ("push_spec",
 	pop_assum SUBST1_TAC >>
 	fs[REPLICATE]
 	) >>
-	
 	xlet `POSTv uv. SEP_EXISTS junk'. qv ~~> Conv NONE [av; iv] * ARRAY av (vvs ++ [xv] ++ junk')`
 	>-(
 		xapp >> xsimpl >> instantiate >> rpt strip_tac >>
@@ -117,25 +133,88 @@ val push_spec = Q.store_thm ("push_spec",
 	xapp >> xsimpl >> rpt strip_tac >>
 	qexists_tac `vvs ++ [xv]` >> qexists_tac `junk'` >>
 	fs[APPEND]
-)
+);
 
+val eq_num_v_thm =
+  mlbasicsProgTheory.eq_v_thm
+  |> DISCH_ALL
+  |> C MATCH_MP (EqualityType_NUM_BOOL |> CONJUNCT1);
 
-
-
-
-
-
-(*DB.find "APPEND" |> DB.find_in "LIST" 
-dest cons
-overload_info_for"++"
-DB.find "LUPDATE" |> DB.find_in "APPEND"
-DB.find "REPLICATE"
-DB.find "LIST_REL" |> DB.find_in "length"
-
-REPLICATE
-	  
-
-DB.find "REPLICATE" |> DB.find_in "LENGTH"
-      DB.find "INT_ADD"*)
+val pop_spec = Q.store_thm("pop_spec",
+  `∀qv.
+   app (p:'ffi ffi_proj) ^(fetch_v "pop" st) [qv]
+     (QUEUE A vs qv)
+     (POST (λv. &(¬NULL vs ∧ A (LAST vs) v) * QUEUE A (FRONT vs) qv)
+           (λe. &(NULL vs ∧ EmptyQueue_exn e) * QUEUE A vs qv))`,
+  xcf "pop" st \\
+  simp[QUEUE_def] >> xpull >>
+  qmatch_abbrev_tac`_ _ frame _` \\
+  xlet `POSTv qr. & (qr = (Conv NONE [av; iv])) * frame`
+  >- ( xapp \\ simp[Abbr`frame`] \\ xsimpl ) \\
+  xmatch \\
+  xlet `POSTv bv. &(BOOL (LENGTH vs = 0) bv) * frame`
+  >- (
+    xapp_spec eq_num_v_thm \\
+    xsimpl \\
+    instantiate ) \\
+  xif
+  >- (
+    xlet `POSTv ev. &EmptyQueue_exn ev * frame`
+    >- (
+      xcon
+      \\ xsimpl
+      \\ simp[EmptyQueue_exn_def] ) \\
+    xraise \\
+    xsimpl \\
+    fs[LENGTH_NIL,NULL_EQ,Abbr`frame`] \\
+    xsimpl) \\
+  xlet `POSTv niv. &(NUM (LENGTH vs - 1) niv) * frame`
+  >- (
+    xapp
+    \\ xsimpl
+    \\ fs[NUM_def]
+    \\ instantiate
+    \\ simp[integerTheory.INT_SUB] )
+  \\ xlet `POSTv xv. &(A (LAST vs) xv) * frame`
+  >- (
+    xapp
+    \\ xsimpl
+    \\ simp[Abbr`frame`]
+    \\ xsimpl
+    \\ instantiate
+    \\ imp_res_tac LIST_REL_LENGTH
+    \\ simp[]
+    \\ `vs ≠ [] ∧ vvs ≠ []` by (rpt strip_tac \\ fs[])
+    \\ `vvs = FRONT vvs ++ [LAST vvs]` by simp[APPEND_FRONT_LAST]
+    \\ pop_assum SUBST1_TAC
+    \\ simp[EL_APPEND1,EL_APPEND2]
+    \\ imp_res_tac list_rel_lastn
+    \\ pop_assum(qspec_then`1`mp_tac)
+    \\ simp[LASTN_1] ) \\
+  xlet `POSTv niv2. &(NUM (LENGTH vs - 1) niv2) * frame`
+  >- (
+    xapp
+    \\ xsimpl
+    \\ fs[NUM_def]
+    \\ instantiate
+    \\ simp[integerTheory.INT_SUB] ) \\
+  xlet `POSTv pv. &(pv = Conv NONE [av; niv2]) * frame`
+  >- ( xcon \\ xsimpl ) \\
+  xlet `POSTv uv. qv ~~> pv * ARRAY av (vvs ++ junk)`
+  >- (
+    xapp
+    \\ simp[Abbr`frame`]
+    \\ xsimpl ) \\
+  xvar
+  >- (
+    xsimpl
+    \\ fs[NULL_EQ,LENGTH_NIL,LENGTH_FRONT,PRE_SUB1]
+    \\ qexists_tac`FRONT vvs`
+    \\ qexists_tac`[LAST vvs] ++ junk`
+    \\ `vvs ≠ []` by (rpt strip_tac \\ fs[])
+    \\ simp[APPEND_FRONT_LAST]
+    \\ fs[LIST_REL_FRONT_LAST] )
+  \\ fs[NULL_EQ,LENGTH_NIL]
+  \\ xsimpl);
 
 val _ = export_theory ()
